remove copy constraint from rot64_bits and abstract away output

Clean/Gadgets/Rotation64/Rotation64Bits.lean
@@ -27,7 +27,7 @@ def rot64_bits (offset : Fin 8) (x : Var U64 (F p)) : Circuit (F p) (Var U64 (F 
   let rotated := highs.zip (lows.rotate 1) |>.map fun (high, low) =>
     high + low * ((2^(8 - offset.val) : ℕ) : F p)
 
-  U64.from_limbs rotated |>.copy
+  return U64.from_limbs rotated
 
 def assumptions (input : U64 (F p)) := input.is_normalized
 
@@ -35,16 +35,21 @@ def spec (offset : Fin 8) (x : U64 (F p)) (y: U64 (F p)) :=
   y.value = rot_right64 x.value offset.val
   ∧ y.is_normalized
 
+def output (offset : Fin 8) (i0 : Nat) : U64 (Expression (F p)) :=
+  U64.from_limbs (.ofFn fun ⟨i,_⟩ =>
+    (var ⟨i0 + i*2 + 1⟩) + var ⟨i0 + (i + 1) % 8 * 2⟩ * .const ((2^(8 - offset.val) : ℕ) : F p))
+
 def elaborated (off : Fin 8) : ElaboratedCircuit (F p) U64 U64 where
   main := rot64_bits off
-  local_length _ := 24
-  output _inputs i0 := var_from_offset U64 (i0 + 16)
+  local_length _ := 16
+  output _ i0 := output off i0
   local_length_eq _ i0 := by
     simp only [circuit_norm, rot64_bits, U64.Copy.circuit,
       ByteDecomposition.circuit, ByteDecomposition.elaborated]
   output_eq _ _ := by
-    simp only [circuit_norm, rot64_bits, U64.Copy.circuit,
-      ByteDecomposition.circuit, ByteDecomposition.elaborated]
+    simp only [circuit_norm, rot64_bits, output, ByteDecomposition.circuit, ByteDecomposition.elaborated]
+    apply congrArg U64.from_limbs
+    simp [Vector.ext_iff, Vector.getElem_rotate]
   subcircuits_consistent _ _ := by
     simp +arith only [circuit_norm, rot64_bits, U64.Copy.circuit,
       ByteDecomposition.circuit, ByteDecomposition.elaborated]
@@ -57,22 +62,18 @@ theorem soundness (offset : Fin 8) : Soundness (F p) (elaborated offset) assumpt
     ByteDecomposition.circuit, ByteDecomposition.elaborated] at h_holds
   simp only [spec, circuit_norm, elaborated, subcircuit_norm, U64.Copy.assumptions, U64.Copy.spec,
     ByteDecomposition.assumptions, ByteDecomposition.spec] at h_holds ⊢
-  set y := eval env (var_from_offset U64 (i0 + 16))
-  obtain ⟨ h_decomposition, h_concatenation ⟩ := h_holds
 
   -- targeted rewriting of the assumptions
-  simp only [size, U64.ByteVector.ext_iff, U64.ByteVector.eval_from_limbs,
-    U64.ByteVector.to_limbs_from_limbs, Vector.getElem_map, Vector.getElem_zip,
-    Vector.getElem_mapIdx, Vector.getElem_rotate, Expression.eval] at h_concatenation
-
   rw [assumptions, U64.ByteVector.is_normalized_iff] at x_normalized
-  simp only [size, Fin.forall_iff, U64.ByteVector.getElem_eval_to_limbs, h_input, x_normalized, true_implies] at h_decomposition
+  simp only [U64.ByteVector.getElem_eval_to_limbs, h_input, x_normalized, true_implies,
+    Fin.forall_iff] at h_holds
 
   set base := ((2^(8 - offset.val) : ℕ) : F p)
   have neg_offset_le : 8 - offset.val ≤ 8 := by
     rw [tsub_le_iff_right, le_add_iff_nonneg_right]; apply zero_le
 
   -- capture the rotation relation in terms of byte vectors
+  set y := eval env (output offset i0)
   set xs := x.to_limbs
   set ys := y.to_limbs
   set o := offset.val
@@ -80,11 +81,12 @@ theorem soundness (offset : Fin 8) : Soundness (F p) (elaborated offset) assumpt
   have h_rot_vector (i : ℕ) (hi : i < 8) :
       ys[i].val < 2^8 ∧
       ys[i].val = xs[i].val / 2^o + (xs[(i + 1) % 8].val % 2^o) * 2^(8-o) := by
-    rw [←h_concatenation i hi]
+    simp only [ys, y, output, U64.ByteVector.eval_from_limbs, U64.ByteVector.to_limbs_from_limbs,
+      Vector.getElem_map, Vector.getElem_ofFn, Expression.eval]
     set high := env.get (i0 + i * 2 + 1)
     set next_low := env.get (i0 + (i + 1) % 8 * 2)
-    have ⟨⟨_, high_eq⟩, ⟨_, high_lt⟩⟩ := h_decomposition i hi
-    have ⟨⟨next_low_eq, _⟩, ⟨next_low_lt, _⟩⟩ := h_decomposition ((i + 1) % 8) (Nat.mod_lt _ (by norm_num))
+    have ⟨⟨_, high_eq⟩, ⟨_, high_lt⟩⟩ := h_holds i hi
+    have ⟨⟨next_low_eq, _⟩, ⟨next_low_lt, _⟩⟩ := h_holds ((i + 1) % 8) (Nat.mod_lt _ (by norm_num))
     have next_low_lt' : next_low.val < 2^(8 - (8 - o)) := by rw [Nat.sub_sub_self offset.is_le']; exact next_low_lt
     have ⟨lt, eq⟩ := byte_decomposition_lt (8-o) neg_offset_le high_lt next_low_lt'
     use lt
